tracing in the innermost loop

src/tidy/rewrite_all.lean
@@ -67,6 +67,10 @@ meta def rewrite_fold {α} (F : expr_lens → expr → α → tactic α) (e : ex
 
 meta def rewrite_F (r : expr × bool) (l : expr_lens) (e : expr) (state : list (expr × expr)) : tactic (list (expr × expr)) := 
 do 
+  e_pp ← pretty_print e,
+  r_pp ← pretty_print r.1,
+  let r_pp := (if r.2 then "← " else "") ++ r_pp,
+  tactic.trace format!"rewritng at {e_pp} via {r_pp}",
   (v, pr) ← rewrite_without_new_mvars r.1 e {symm := r.2},
   let v' := l.replace v,
   pr' ← l.congr pr,
@@ -81,14 +85,15 @@ def remove_adjacent_duplicates {α β} (f : α → β) [decidable_eq β] : list 
 | [] := []
 
 meta def all_rewrites (r : expr × bool) (e : expr) : tactic (list (expr × expr)) :=
-do pp ← pretty_print e,
+do 
+  --  pp ← pretty_print e,
    results ← rewrite_fold (rewrite_F r) e [],
    let results : list (expr × expr) := remove_adjacent_duplicates (λ p, p.1) results,
-   results_pp ← results.mmap(λ p, pretty_print p.1),
-   r_pp ← pretty_print r.1,
-   let r_pp := (if r.2 then "← " else "") ++ r_pp,
-   tactic.trace format!"⟫ finding all rewrites of {pp} via {r_pp}",
-   results_pp.mmap'(λ r, tactic.trace format!"⟫⟫ {r}"),
+  --  results_pp ← results.mmap(λ p, pretty_print p.1),
+  --  r_pp ← pretty_print r.1,
+  --  let r_pp := (if r.2 then "← " else "") ++ r_pp,
+  --  tactic.trace format!"⟫ finding all rewrites of {pp} via {r_pp}",
+  --  results_pp.mmap'(λ r, tactic.trace format!"⟫⟫ {r}"),
    pure results
 
 meta def perform_nth_rewrite (r : expr × bool) (n : ℕ) : tactic unit := 
@@ -112,11 +117,11 @@ do e ← target,
    (new_t, prf) ← rewrites.nth n,
    replace_target new_t prf
 
--- @[search] lemma b (l : list ℕ) : 1 :: l = 2 :: l := sorry
+@[search] lemma b (l : list ℕ) : 1 :: l = 2 :: l := sorry
 
--- example (f : ℕ → list ℕ → Type) : f 3 [1,1,1,2,1] = f 3 [1,2,1,2,1] :=
--- begin
--- target >>= all_rewrites_using `search,
--- perform_nth_rewrite_using `search 5,
--- refl
--- end
+example (f : ℕ → list ℕ → Type) : f 3 [1,1,1,2,1] = f 3 [1,2,1,2,1] :=
+begin
+target >>= all_rewrites_using `search,
+perform_nth_rewrite_using `search 5,
+refl
+end
